proof/eclib/IntDiv_extra.ec
@@ -21,13 +21,15 @@ proof. by rewrite /vp; apply/ge0_argmax. qed.
 
 lemma vp_pow_dvd b x : 1 < b => x <> 0 => (b ^ (vp b x)) %| x.
 proof.
-by move => lt1b neqx0; rewrite /vp; apply/(argmaxP ((^) b) (transpose (%|) x) 0 `|x| _ _ _ _) => //=;
-[apply/normr_ge0|rewrite expr0 dvd1z|apply vp_bound].
+move => lt1b neqx0; rewrite /vp; apply/(argmaxP ((^) b) (transpose (%|) x) 0 `|x| _ _ _ _) => //=;
+[apply/normr_ge0|apply vp_bound].
+assumption.
+assumption.
 qed.
 
 lemma vp0 b x : 1 < b => x <> 0 => x %% b <> 0 => vp b x = 0.
 proof.
-rewrite -dvdzE /vp => lt1b neqx0 Ndvdbx; apply argmax_eq => //=; first by rewrite expr0 dvd1z.
+rewrite -dvdzE /vp => lt1b neqx0 Ndvdbx; apply argmax_eq => //=.
 by move=> j /ltzE /= le1j; move: Ndvdbx; apply/implybNN/dvdz_trans; move: (dvdz_exp2l b 1 j); rewrite expr1 le1j.
 qed.
 
